packages/logic/Gimlight/Logic/Position.lean
@@ -8,11 +8,4 @@ namespace Gimlight
 public def Position.inBounds (map : Map) (position : Position) : Prop :=
   position.x < map.dimensions.width ∧ position.y < map.dimensions.height
 
-public def Position.step (direction : Direction) (position : Position) : Option Position :=
-  match direction with
-  | .left => if position.x = 0 then none else some { position with x := position.x - 1 }
-  | .right => some { position with x := position.x + 1 }
-  | .up => if position.y = 0 then none else some { position with y := position.y - 1 }
-  | .down => some { position with y := position.y + 1 }
-
 end Gimlight
