packages/logic/Gimlight/Logic/Position/Basic.lean
@@ -1,10 +1,19 @@
 module
 
+public import Gimlight.Logic.Direction
+
 namespace Gimlight
 
 public structure Position where
   x : Nat
   y : Nat
 deriving DecidableEq, Repr
+
+@[expose] public def Position.step (direction : Direction) (position : Position) : Option Position :=
+  match direction with
+  | .left => if position.x = 0 then none else some { position with x := position.x - 1 }
+  | .right => some { position with x := position.x + 1 }
+  | .up => if position.y = 0 then none else some { position with y := position.y - 1 }
+  | .down => some { position with y := position.y + 1 }
 
 end Gimlight
